LeanStlc/Preservation.lean
@@ -17,8 +17,8 @@ def Typing.preservation_step : Γ ⊢ t : A -> t ~> t' -> Γ ⊢ t' : A
 | nrec z s n, .nrec3 r => nrec z s (n.preservation_step r)
 | inl t, .inl r => inl (t.preservation_step r)
 | inr t, .inr r => inr (t.preservation_step r)
-| case (inl h1) h2 h3, .case_inl => beta h2 h1
-| case (inr h1) h2 h3, .case_inr => beta h3 h1
+| case (inl h1) h2 h3, .case_inl => Typing.app h2 h1
+| case (inr h1) h2 h3, .case_inr => Typing.app h3 h1
 | case h1 h2 h3, .case1 r => Typing.case (Typing.preservation_step h1 r) h2 h3
 | case h1 h2 h3, .case2 r => Typing.case h1 (Typing.preservation_step h2 r) h3
 | case h1 h2 h3, .case3 r => Typing.case h1 h2 (Typing.preservation_step h3 r)
