LeanStlc/StrongNorm4.lean
@@ -24,9 +24,9 @@ mutual
   | succ : SnNor Γ S t -> SnNor Γ S t.succ
   | neu : SnNeu Γ S t -> SnNor Γ S t
   | red : SnRed Γ S t t' -> SnNor Γ S t' -> SnNor Γ S t
-  | inl : SnNor S1 Γ t -> SnNor S2 Γ t.inl
-  | inr : SnNor S1 Γ t -> SnNor S2 Γ t.inr
-  | pair : SnNor S1 Γ a -> SnNor S2 Γ b -> SnNor S3 Γ (.pair a b)
+  | inl : ℛ S2 Γ t.inl -> SnNor S1 Γ t -> SnNor S2 Γ t.inl
+  | inr : ℛ S2 Γ t.inr -> SnNor S1 Γ t -> SnNor S2 Γ t.inr
+  | pair : ℛ S3 Γ (.pair a b) -> SnNor S1 Γ a -> SnNor S2 Γ b -> SnNor S3 Γ (.pair a b)
   | tt : SnNor Γ S .tt
 
   @[grind]
@@ -36,7 +36,7 @@ mutual
   | nrec : SnNor S1 Γ z -> SnNor S2 Γ s -> SnNeu S3 Γ t -> SnNeu S4 Γ (.nrec A z s t)
   | fst : SnNeu S1 Γ t -> SnNeu S2 Γ t.fst
   | snd : SnNeu S1 Γ t -> SnNeu S2 Γ t.snd
-  | case : SnNeu S1 Γ d -> SnNor S2 (A :: Γ) a -> SnNor S2 (A :: Γ) b -> SnNeu S2 Γ (.case A d a b)
+  | case : SnNeu S1 Γ d -> SnNor S2 Γ a -> SnNor S3 Γ b -> SnNeu S4 Γ (.case A d a b)
 
   @[grind]
   inductive SnRed : CtxSet -> CtxRel
@@ -47,8 +47,11 @@ mutual
   | step_nrec : SnRed S1 Γ n n' -> SnRed S2 Γ (.nrec A z s n) (.nrec A z s n')
   | fst : SnNor S1 Γ b -> SnRed S2 Γ (.fst (.pair a b)) a
   | snd : SnNor S1 Γ a -> SnRed S2 Γ (.snd (.pair a b)) b
-  | inl : SnNor S1 Γ1 b -> SnRed S2 (A :: Γ2) (.case A (.inl t) a b) a[su t :: +0]
-  | inr : SnNor S1 Γ1 a -> SnRed S2 (A :: Γ2) (.case A (.inr t) a b) b[su t :: +0]
+  | inl : SnNor S1 Γ b -> SnRed S2 Γ (.case A (.inl t) a b) (a :@ t)
+  | inr : SnNor S1 Γ a -> SnRed S2 Γ (.case A (.inr t) a b) (b :@ t)
+  | step_case : SnRed S1 Γ d d' -> SnRed S2 Γ (.case A d a b) (.case A d' a b)
+  | step_fst : SnRed S1 Γ t t' -> SnRed S2 Γ (t.fst) (t'.fst)
+  | step_snd : SnRed S1 Γ t t' -> SnRed S2 Γ (t.snd) (t'.snd)
 end
 
 theorem SnRed.preservation : Γ ⊢ t : A -> SnRed S Γ t t' -> Γ ⊢ t' : A
@@ -59,8 +62,12 @@ theorem SnRed.preservation : Γ ⊢ t : A -> SnRed S Γ t t' -> Γ ⊢ t' : A
 | Typing.nrec j1 j2 j3, .step_nrec h1 => Typing.nrec j1 j2 (SnRed.preservation j3 h1)
 | Typing.fst (Typing.pair j1 _), fst j3 => j1
 | Typing.snd (Typing.pair _ j2), snd j3 => j2
-| Typing.case (.inl h1) h2 h3, inl h4 => Typing.beta h2 h1
-| Typing.case (.inr h1) _ h3, inr h5 => Typing.beta h3 h1
+| Typing.case (.inl h1) h2 _, inl h4 => Typing.app h2 h1
+| Typing.case (.inr h1) _ h3, inr h5 => Typing.app h3 h1
+| Typing.case h1 h2 h3, .step_case h4 => Typing.case (SnRed.preservation h1 h4) h2 h3
+| Typing.fst j1, .step_fst h => Typing.fst (SnRed.preservation j1 h)
+| Typing.snd j1, .step_snd h => Typing.snd (SnRed.preservation j1 h)
+| _, _ => sorry
 
 mutual
   theorem SnNor.rename (m : Γ -⟨r⟩> Δ) : SnNor S Γ t -> SnNor S Δ t[r]
@@ -72,9 +79,9 @@ mutual
   | .succ t => .succ (t.rename m)
   | .neu t => .neu (t.rename m)
   | .red h t' => .red (h.rename m) (t'.rename m)
-  | .inl t => .inl (t.rename m)
-  | .inr t => .inr (t.rename m)
-  | .pair h1 h2 => .pair (h1.rename m) (h2.rename m)
+  | .inl h t => .inl (by intro r Δ' h'; sorry) (t.rename m)
+  | .inr h t => .inr sorry (t.rename m)
+  | .pair h h1 h2 => .pair sorry (h1.rename m) (h2.rename m)
   | .tt => .tt
 
   theorem SnNeu.rename (m : Γ -⟨r⟩> Δ) : SnNeu S Γ t -> SnNeu S Δ t[r]
@@ -82,9 +89,7 @@ mutual
   | .app s t => .app (s.rename m) (t.rename m)
   | .nrec t z s => .nrec (t.rename m) (z.rename m) (s.rename m)
   | .case (A := A) h1 h2 h3 =>
-    have lem1 := SnNeu.rename (m.lift A) h2
-    have lem2 := SnNeu.rename (m.lift A) h3
-    .case (h1.rename m) (sorry) (sorry)
+    .case (h1.rename m) (h2.rename m) (h3.rename m)
   | .snd h => .snd (h.rename m)
   | .fst h => .fst (h.rename m)
 
@@ -99,8 +104,11 @@ mutual
   | .step_nrec h => .step_nrec (h.rename m)
   | .fst h => .fst (h.rename m)
   | .snd h => .snd (h.rename m)
-  | .inl h => sorry
-  | .inr h => sorry
+  | .inl h => .inl (h.rename m)
+  | .inr h => .inr (h.rename m)
+  | .step_case h => .step_case (h.rename m)
+  | .step_fst h => .step_fst (h.rename m)
+  | .step_snd h => .step_snd (h.rename m)
 end
 
 @[simp]
@@ -109,9 +117,14 @@ def 𝒱 : Ty -> CtxSet
   λ Γ x => match x with
   | :λ[_] t => ∀ a, Γ ⊢ a : A -> SnNor (𝒱 A) Γ a -> (A :: Γ) ⊢ t : B -> SnNor (𝒱 B) Γ t[su a::+0]
   | _ => False
-| .plus A B => --unnecessary?
+| .plus A B =>
   λ Γ x => match x with
-  | .inl t => (Γ ⊢ t : A ∧ SnNor (𝒱 A) Γ t) ∨ (Γ ⊢ t : B ∧ SnNor (𝒱 B) Γ t)
+  | .inl t => (Γ ⊢ t : A ∧ SnNor (𝒱 A) Γ t)
+  | .inr t => (Γ ⊢ t : B ∧ SnNor (𝒱 B) Γ t)
+  | _ => False
+| .product A B =>
+  λ Γ x => match x with
+  | .pair a b => (Γ ⊢ a : A ∧ SnNor (𝒱 A) Γ a) ∧ (Γ ⊢ b : B ∧ SnNor (𝒱 B) Γ b)
   | _ => False
 | _ => CtxSet.empty
 
@@ -178,22 +191,43 @@ theorem ℰ.nrec :
   SnNor S Γ n ->
   ℰ Γ A (.nrec A z s n)
 | ⟨j1, j2⟩, ⟨j3, j4⟩, _, j5, .zero => ⟨Typing.nrec j1 j3 j5, SnNor.red (SnRed.zero _ j4) j2⟩
-| ⟨j1, j2⟩, ⟨j3, j4⟩, eq, Typing.succ j5, .succ h1 => ⟨Typing.nrec j1 j3 (Typing.succ j5) , SnNor.red (SnRed.succ) (SnNor.appl rfl j3 j4 (ℰ.nrec ⟨j1, j2⟩ ⟨j3, j4⟩ eq j5 h1)).2⟩
+| ⟨j1, j2⟩, ⟨j3, j4⟩, eq, Typing.succ j5, .succ h1 => ⟨Typing.nrec j1 j3 (Typing.succ j5), SnNor.red (SnRed.succ) (SnNor.appl rfl j3 j4 (ℰ.nrec ⟨j1, j2⟩ ⟨j3, j4⟩ eq j5 h1)).2⟩
 | ⟨j1, j2⟩, ⟨j3, j4⟩, _, j5, .neu h1 => ⟨Typing.nrec j1 j3 j5, SnNor.neu (SnNeu.nrec j2 j4 h1)⟩
 | ⟨j1, j2⟩, ⟨j3, j4⟩, eq, j5, .red h1 h2 => ⟨Typing.nrec j1 j3 j5, SnNor.red (SnRed.step_nrec h1) (ℰ.nrec ⟨j1, j2⟩ ⟨j3,j4⟩ eq (SnRed.preservation j5 h1) h2).2⟩
-| ⟨j1, j2⟩, ⟨j3, j4⟩, _, j5, .inl h => ⟨Typing.nrec j1 j3 j5, sorry⟩
-| ⟨j1, j2⟩, ⟨j3, j4⟩, _, j5, .inr h => ⟨Typing.nrec j1 j3 j5, sorry⟩
 
 theorem ℰ.case:
   S = 𝒱 (.plus A B) ->
   Γ ⊢ d : (.plus A B) ->
   SnNor S Γ d ->
-  ℰ (A :: Γ) C a ->
-  ℰ (B :: Γ) C b ->
+  ℰ Γ (A -t> C) a ->
+  ℰ Γ (B -t> C) b ->
   ℰ Γ C (Term.case C d a b)
-| eq, Typing.inl j1, j2, ⟨j3, j4⟩, ⟨j5, j6⟩ => ⟨Typing.case (Typing.inl j1) j3 j5, SnNor.red (SnRed.inl j6) sorry⟩
-| eq, j1, j2, ⟨j3, j4⟩, ⟨j5, j6⟩ => ⟨Typing.case (sorry) j3 j5, sorry⟩
+| eq, Typing.inl j1, SnNor.inl h j2, ⟨j3, j4⟩, ⟨j5, j6⟩ =>
+  ⟨Typing.case (Typing.inl j1) j3 j5,
+   SnNor.red (SnRed.inl j6) (SnNor.appl rfl j3 j4 ⟨j1, (by subst eq; simp only [ℛ] at h; replace h := @h id Γ TypingRen.id; simp at h; apply h.2)⟩).2⟩
+| eq, Typing.inr j1, SnNor.inr h j2, ⟨j3, j4⟩, ⟨j5, j6⟩ =>
+  ⟨Typing.case (Typing.inr j1) j3 j5,
+   SnNor.red (SnRed.inr j4) (SnNor.appl rfl j5 j6 ⟨j1, (by subst eq; simp only [ℛ] at h; replace h := @h id Γ TypingRen.id; simp at h; apply h.2)⟩).2⟩
+| eq, j1, SnNor.neu j2, ⟨j3, j4⟩, ⟨j5, j6⟩ => ⟨Typing.case j1 j3 j5, SnNor.neu (SnNeu.case j2 j4 j6)⟩
+| eq, j1, SnNor.red h j2, ⟨j3, j4⟩, ⟨j5, j6⟩ => ⟨Typing.case j1 j3 j5, SnNor.red (SnRed.step_case h) (ℰ.case eq (SnRed.preservation j1 h) j2 ⟨j3, j4⟩ ⟨j5, j6⟩ ).2⟩
 
+theorem ℰ.fst :
+  S = 𝒱 (.product A B) ->
+  Γ ⊢ t : (.product A B) ->
+  SnNor S Γ t ->
+  SnNor (𝒱 A) Γ t.fst
+| eq, Typing.pair j1 j2, SnNor.pair h h1 h2 => SnNor.red (SnRed.fst h2) (by subst eq;simp only [ℛ] at h; replace h := @h id Γ TypingRen.id; simp at h; apply h.1.2)
+| eq, j1, SnNor.neu j2 => SnNor.neu (SnNeu.fst j2)
+| eq, j1, SnNor.red h j2 => SnNor.red (SnRed.step_fst h) (ℰ.fst rfl (SnRed.preservation j1 h) (by rw [eq] at j2; apply j2))
+
+theorem ℰ.snd :
+  S = 𝒱 (.product A B) ->
+  Γ ⊢ t : (.product A B) ->
+  SnNor S Γ t ->
+  SnNor (𝒱 B) Γ t.snd
+| eq, Typing.pair j1 j2, SnNor.pair h h1 h2 => SnNor.red (SnRed.snd h2) (by subst eq;simp only [ℛ] at h; replace h := @h id Γ TypingRen.id; simp at h; apply h.2.2)
+| eq, j1, SnNor.neu j2 => SnNor.neu (SnNeu.snd j2)
+| eq, j1, SnNor.red h j2 => SnNor.red (SnRed.step_fst h) (ℰ.fst rfl (SnRed.preservation j1 h) (by rw [eq] at j2; apply j2))
 
 theorem fundamental : Γ ⊢ t : A -> Γ ⊨ t : A
 | .var xj, σ, Δ, h => h.act xj
@@ -216,28 +250,31 @@ theorem fundamental : Γ ⊢ t : A -> Γ ⊨ t : A
   let sj' := fundamental sj h
   let nj' := fundamental nj h
   ℰ.nrec zj' sj' rfl nj'.1 nj'.2
-| .inl nj, σ, Δ, h =>
-  let nj' := fundamental nj h
-  ⟨Typing.inl nj'.1, SnNor.inl nj'.2⟩
-| .inr nj, σ, Δ, h =>
-  let nj' := fundamental nj h
-  ⟨Typing.inr nj'.1, SnNor.inr nj'.2⟩
+| .inl (t := t) (A := A) (B := B) nj, σ, Δ, h =>
+  let nj' : Γ ⊨ t : A := fundamental nj
+  have lem1 {Δ' r} : Δ -⟨r⟩> Δ' -> 𝒱 (.plus A B) Δ' (Term.inl t[σ][r.to]) :=  λ h1 =>
+    ⟨(nj' (SemSubst.compose h h1)).1 |> cast (by simp), (nj' (SemSubst.compose h h1)).2 |> cast (by simp)⟩
+  ⟨Typing.inl (nj' h).1, SnNor.inl lem1 (nj' h).2⟩
+| .inr (t := t) (A := A) (B := B) nj, σ, Δ, h =>
+  let nj' : Γ ⊨ t : B := fundamental nj
+  have lem1 {Δ' r} : Δ -⟨r⟩> Δ' -> 𝒱 (.plus A B) Δ' (Term.inr t[σ][r.to]) :=  λ h1 =>
+  ⟨(nj' (SemSubst.compose h h1)).1 |> cast (by simp), (nj' (SemSubst.compose h h1)).2 |> cast (by simp)⟩
+  ⟨Typing.inr (nj' h).1, SnNor.inr lem1 (nj' h).2⟩
 | .case (A := A) (B := B) (C := C) h1 h2 h3, σ, Δ, h =>
   let h1' := fundamental h1 h
-  let lem := SemSubst.lift h
-  let h2' := fundamental h2 (lem A)
-  let h3' := fundamental h3 (lem B)
-  (ℰ.case h1' h2' h3')
+  let h2' := fundamental h2 h
+  let h3' := fundamental h3 h
+  (ℰ.case rfl h1'.1 h1'.2 h2' h3')
 | .fst nj, σ, Δ, h =>
   let nj' := fundamental nj h
-  ⟨Typing.fst nj'.1, sorry⟩
+  ⟨Typing.fst nj'.1, (ℰ.fst rfl nj'.1 nj'.2)⟩
 | .snd nj, σ, Δ, h =>
   let nj' := fundamental nj h
   ⟨Typing.snd nj'.1, sorry⟩
 | .pair h1 h2, σ, Δ, h =>
   let h1' := fundamental h1 h
   let h2' := fundamental h2 h
-  ⟨Typing.pair h1'.1 h2'.1, SnNor.pair h1'.2 h2'.2⟩
+  ⟨Typing.pair h1'.1 h2'.1, SnNor.pair sorry h1'.2 h2'.2⟩
 | .tt, σ, Δ, h => ⟨Typing.tt, SnNor.tt⟩
 
 end StrongNormalization4
